Minor refactoring of BitMachine and translation.

Coq/Simplicity/BitMachine.v
@@ -27,18 +27,6 @@ Definition newWriteFrame n : WriteFrame := {| writeData := nil; writeEmpty := n 
  *)
 Definition fullWriteFrame l : WriteFrame := {| writeData := rev l; writeEmpty := 0 |}.
 
-Definition writeToFrame v f : option WriteFrame :=
-match writeEmpty f with
-| O => None
-| (S n) => Some {| writeData := v :: writeData f; writeEmpty := n |}
-end.
-
-Fixpoint writeListFrame l f : option WriteFrame :=
-match l with
-| nil => Some f
-| hd :: tl => option_bind (writeListFrame tl) (writeToFrame hd f)
-end.
-
 (* Read-only frames are represented in zipper format.  The cells before the
  * cursor are stored in prevData in reverse order.  The cells after the cursor
  * are stored in nextData in forward order.
@@ -50,10 +38,7 @@ Record ReadFrame :=
 
 Definition readSize rf := length (prevData rf) + length (nextData rf).
 
-Definition setFrame l :=
- {| prevData := nil
-  ; nextData := l
-  |}.
+Definition setFrame l := {| prevData := nil; nextData := l |}.
 
 (* The full state of the Bit Machine is captured by a list of inactive
  * read-only and write-only frames.  The top of the two stacks are held in the
@@ -73,10 +58,10 @@ repeat (decide equality).
 Qed.
 
 Definition stateSize s :=
-  fold_right plus 0 (map readSize (inactiveReadFrames s)) +
+  nat_sum (map readSize (inactiveReadFrames s)) +
   readSize (activeReadFrame s) +
   writeSize (activeWriteFrame s) +
-  fold_right plus 0 (map writeSize (inactiveWriteFrames s)).
+  nat_sum (map writeSize (inactiveWriteFrames s)).
 
 (* Logically, the state of the Bit Machine is commonly divided between the part
  * of the state that we are focused on and the rest of state.  The focused part
@@ -159,6 +144,9 @@ Definition fillReadFrame (ctx : Context) (h : ReadFrame) : State :=
 
 Module MachineCode.
 
+(* This machine code type specifies all legal basic Bit Machine state
+ * transitions.
+ *)
 Inductive T : State -> State -> Set :=
 | NewFrame : forall n ctx,
     T ctx
@@ -223,7 +211,15 @@ Inductive T : State -> State -> Set :=
 
 End MachineCode.
 
-Definition MoveFrame_ctx s :
+(* For each basic instruction we define function to check if a given state s is
+ * valid state that the instruction can execute in.  If it is valid we return
+ * a witness proving that s can be expressed in the form of a valid state. Each
+ * function also has a correctness function that proves that any state that is
+ * in the form of a valid state, the check function return success.  The
+ * NewFrame instruction is valid in every state and therefore doesn't have a
+ * check function.
+ *)
+Definition MoveFrame_chk s :
   option { lctx : list Cell * Context | let (l, ctx) := lctx in s =
       {| inactiveReadFrames := inactiveReadFrames ctx
        ; activeReadFrame := activeReadFrame ctx
@@ -244,7 +240,7 @@ unfold fullWriteFrame.
 abstract (rewrite rev_involutive; reflexivity).
 Defined.
 
-Lemma MoveFrame_ctx_correct l ctx : MoveFrame_ctx
+Lemma MoveFrame_chk_correct l ctx : MoveFrame_chk
  {| inactiveReadFrames := inactiveReadFrames ctx
   ; activeReadFrame := activeReadFrame ctx
   ; activeWriteFrame := fullWriteFrame l
@@ -252,7 +248,7 @@ Lemma MoveFrame_ctx_correct l ctx : MoveFrame_ctx
   |} = Some (exist _ (l, ctx) (refl_equal _)).
 Proof.
 cbn.
-set (H := (MoveFrame_ctx_subproof _ _ _ _ _)).
+set (H := (MoveFrame_chk_subproof _ _ _ _ _)).
 generalize H; clear H.
 rewrite (rev_involutive l).
 apply (K_dec_set State_dec).
@@ -260,7 +256,7 @@ destruct ctx as [irf arf awf iwf].
 reflexivity.
 Qed.
 
-Definition DropFrame_ctx s :
+Definition DropFrame_chk s :
   option { rfctx : ReadFrame * Context | let (rf, ctx) := rfctx in s =
       {| inactiveReadFrames := activeReadFrame ctx :: inactiveReadFrames ctx
        ; activeReadFrame := rf
@@ -269,17 +265,16 @@ Definition DropFrame_ctx s :
        |}}.
 destruct s as [[|arf irf] rf awf iwf].
  exact None.
-pose (ctx := {| inactiveReadFrames := irf
-              ; activeReadFrame := arf
-              ; activeWriteFrame := awf
-              ; inactiveWriteFrames := iwf
-              |}).
 left.
-exists (rf, ctx).
+exists (rf, {| inactiveReadFrames := irf
+             ; activeReadFrame := arf
+             ; activeWriteFrame := awf
+             ; inactiveWriteFrames := iwf
+             |}).
 reflexivity.
 Defined.
 
-Lemma DropFrame_ctx_correct rf ctx : DropFrame_ctx
+Lemma DropFrame_chk_correct rf ctx : DropFrame_chk
  {| inactiveReadFrames := activeReadFrame ctx :: inactiveReadFrames ctx
   ; activeReadFrame := rf
   ; activeWriteFrame := activeWriteFrame ctx
@@ -289,7 +284,7 @@ Proof.
 destruct ctx; reflexivity.
 Qed.
 
-Definition Write_ctx s :
+Definition Write_chk s :
   option { ctx : Context | s =
     fillContext ctx {| readLocalState := nil
                      ; writeLocalState := newWriteFrame 1
@@ -297,16 +292,15 @@ Definition Write_ctx s :
 destruct s as [irf [rp rn] [wd [|we]] iwf].
  exact None.
 left.
-pose (ctx := {| inactiveReadFrames := irf
-              ; activeReadFrame := {| prevData := rp; nextData := rn |}
-              ; activeWriteFrame := {| writeData := wd; writeEmpty := we |}
-              ; inactiveWriteFrames := iwf
-              |}).
-exists ctx.
+exists {| inactiveReadFrames := irf
+        ; activeReadFrame := {| prevData := rp; nextData := rn |}
+        ; activeWriteFrame := {| writeData := wd; writeEmpty := we |}
+        ; inactiveWriteFrames := iwf
+        |}.
 reflexivity.
 Defined.
 
-Lemma Write_ctx_correct ctx : Write_ctx
+Lemma Write_chk_correct ctx : Write_chk
   (fillContext ctx {| readLocalState := nil
                     ; writeLocalState := newWriteFrame 1
                     |})
@@ -316,7 +310,7 @@ destruct ctx as [irf [rp rn] [wd we] iwf].
 reflexivity.
 Qed.
 
-Definition Skip_ctx n s :
+Definition Skip_chk n s :
   option { ctx : Context | s =
     fillContext ctx {| readLocalState := nil
                      ; writeLocalState := newWriteFrame n
@@ -338,7 +332,7 @@ abstract (
   reflexivity).
 Defined.
 
-Lemma Skip_ctx_correct n ctx : Skip_ctx n
+Lemma Skip_chk_correct n ctx : Skip_chk n
   (fillContext ctx {| readLocalState := nil
                     ; writeLocalState := newWriteFrame n
                     |})
@@ -347,7 +341,7 @@ Proof.
 cbn.
 destruct (Nat.leb_spec n (n + writeEmpty (activeWriteFrame ctx))) as [H0|H0];
  [|elim (Lt.lt_not_le _ _ H0); auto with arith].
-set (H := (Skip_ctx_subproof _ _ _ _ _ _ _ _)).
+set (H := (Skip_chk_subproof _ _ _ _ _ _ _ _)).
 generalize H; clear H.
 rewrite Minus.minus_plus.
 apply (K_dec_set State_dec).
@@ -355,7 +349,7 @@ destruct ctx as [irf [rp rn] [wd we] iwf].
 reflexivity.
 Qed.
 
-Definition Copy_ctx n s :
+Definition Copy_chk n s :
   option { lctx : list Cell * Context | let (l, ctx) := lctx in n = length l /\ s =
     fillContext ctx {| readLocalState := l
                      ; writeLocalState := newWriteFrame (length l)
@@ -387,7 +381,7 @@ split.
  reflexivity).
 Defined.
 
-Lemma Copy_ctx_correct l ctx : Copy_ctx (length l)
+Lemma Copy_chk_correct l ctx : Copy_chk (length l)
   (fillContext ctx {| readLocalState := l
                     ; writeLocalState := newWriteFrame (length l)
                     |})
@@ -398,23 +392,18 @@ destruct (Nat.leb_spec (length l) (length l + writeEmpty (activeWriteFrame ctx))
  [|elim (Lt.lt_not_le _ _ H0); auto with arith].
 destruct (Nat.leb_spec (length l) (length (l ++ nextData (activeReadFrame ctx)))) as [H1|H1];
  [|elim (Lt.lt_not_le _ _ H1); rewrite app_length; auto with arith].
-set (H := (Copy_ctx_subproof _ _ _)).
+set (H := (Copy_chk_subproof _ _ _)).
 generalize H; clear H.
-set (H := (Copy_ctx_subproof0 _ _ _ _ _ _ _ _ _)).
+set (H := (Copy_chk_subproof0 _ _ _ _ _ _ _ _ _)).
 generalize H; clear H.
-rewrite firstn_app, firstn_all, Nat.sub_diag; cbn.
-rewrite app_nil_r, Minus.minus_plus.
-replace (skipn (length l) _) with (nextData (activeReadFrame ctx))
- by (apply (app_inv_head (firstn (length l) (l ++ nextData (activeReadFrame ctx))));
-     rewrite firstn_skipn, firstn_app, firstn_all, Nat.sub_diag; cbn;
-     rewrite app_nil_r; reflexivity).
+rewrite firstn_app_3, Minus.minus_plus, skipn_app_3.
 intros H; elim H using (K_dec_set State_dec); clear H.
 apply (K_dec_set Nat.eq_dec).
 destruct ctx as [irf [rp rn] [wd we] iwf].
 reflexivity.
 Qed.
 
-Definition Fwd_ctx n s :
+Definition Fwd_chk n s :
   option { lctx : list Cell * Context | let (l, ctx) := lctx in n = length l /\ s =
     fillReadFrame ctx {| prevData := nil
                        ; nextData := l
@@ -429,19 +418,19 @@ pose (ctx := {| inactiveReadFrames := irf
               ; inactiveWriteFrames := iwf
               |}).
 exists (firstn n rn, ctx).
-split.
-- abstract
-(inversion_clear Hrn as [H|];
+abstract(
+split;[
+ inversion_clear Hrn as [H|];
  rewrite (firstn_length_le _ H);
- reflexivity).
-- abstract
-(unfold fillReadFrame; cbn;
+ reflexivity
+|unfold fillReadFrame; cbn;
  inversion_clear Hrn as [H|];
  rewrite firstn_skipn;
- reflexivity).
+ reflexivity
+]).
 Defined.
 
-Lemma Fwd_ctx_correct l ctx : Fwd_ctx (length l)
+Lemma Fwd_chk_correct l ctx : Fwd_chk (length l)
   (fillReadFrame ctx {| prevData := nil
                       ; nextData := l
                       |})
@@ -450,23 +439,18 @@ Proof.
 cbn.
 destruct (Nat.leb_spec (length l) (length (l ++ nextData (activeReadFrame ctx)))) as [H0|H0];
  [|elim (Lt.lt_not_le _ _ H0); rewrite app_length; auto with arith].
-set (H := (Fwd_ctx_subproof _ _ _)).
+set (H := (Fwd_chk_subproof _ _ _ _ _ _ _)).
 generalize H; clear H.
-set (H := (Fwd_ctx_subproof0 _ _ _ _ _ _ _)).
-generalize H; clear H.
-rewrite firstn_app, firstn_all, Nat.sub_diag; cbn.
-rewrite app_nil_r.
-replace (skipn (length l) _) with (nextData (activeReadFrame ctx))
- by (apply (app_inv_head (firstn (length l) (l ++ nextData (activeReadFrame ctx))));
-     rewrite firstn_skipn, firstn_app, firstn_all, Nat.sub_diag; cbn;
-     rewrite app_nil_r; reflexivity).
-intros H; elim H using (K_dec_set State_dec); clear H.
-apply (K_dec_set Nat.eq_dec).
+rewrite firstn_app_3, skipn_app_3.
+intros [eq0 eq1].
+elim eq0 using (K_dec_set Nat.eq_dec).
+elim eq1 using (K_dec_set State_dec).
+clear eq0 eq1.
 destruct ctx as [irf [rp rn] [wd we] iwf].
 reflexivity.
 Qed.
 
-Definition Bwd_ctx n s :
+Definition Bwd_chk n s :
   option { lctx : list Cell * Context | let (l, ctx) := lctx in n = length l /\ s =
     fillReadFrame ctx {| prevData := rev l
                        ; nextData := nil
@@ -481,19 +465,18 @@ pose (ctx := {| inactiveReadFrames := irf
               ; inactiveWriteFrames := iwf
               |}).
 exists (rev (firstn n rp), ctx).
-split.
-- abstract
-(inversion_clear Hrp as [H|];
+abstract(split;
+[inversion_clear Hrp as [H|];
  rewrite rev_length, (firstn_length_le _ H);
- reflexivity).
-- abstract
-(unfold fillReadFrame; cbn;
+ reflexivity
+|unfold fillReadFrame; cbn;
  inversion_clear Hrp as [H|];
  rewrite rev_involutive, firstn_skipn;
- reflexivity).
+ reflexivity
+]).
 Defined.
 
-Lemma Bwd_ctx_correct l ctx : Bwd_ctx (length l)
+Lemma Bwd_chk_correct l ctx : Bwd_chk (length l)
   (fillReadFrame ctx {| prevData := rev l
                       ; nextData := nil
                       |})
@@ -502,22 +485,17 @@ Proof.
 cbn.
 destruct (Nat.leb_spec (length l) (length (rev l ++ prevData (activeReadFrame ctx)))) as [H0|H0];
  [|elim (Lt.lt_not_le _ _ H0); rewrite app_length, rev_length; auto with arith].
-set (H := (Bwd_ctx_subproof _ _ _)).
+set (H := (Bwd_chk_subproof _ _ _ _ _ _ _)).
 generalize H; clear H.
-set (H := (Bwd_ctx_subproof0 _ _ _ _ _ _ _)).
-generalize H; clear H.
-rewrite firstn_app.
-replace (firstn (length l) (rev l)) with (rev l) by
- (rewrite <- rev_length, firstn_all; reflexivity).
-replace (firstn (length l - length (rev l)) _) with (@nil Cell) by
- (rewrite rev_length, Nat.sub_diag; reflexivity).
-replace (skipn (length l) _) with (prevData (activeReadFrame ctx)) by
- (apply (app_inv_head (firstn (length l) (rev l ++ prevData (activeReadFrame ctx))));
-  rewrite <- rev_length, firstn_skipn, firstn_app, firstn_all, Nat.sub_diag; cbn;
-  rewrite app_nil_r; reflexivity).
-rewrite app_nil_r, (rev_involutive l).
-intros H; elim H using (K_dec_set State_dec); clear H.
-apply (K_dec_set Nat.eq_dec).
+replace (firstn (length l)) with (@firstn Cell (length (rev l))) by
+  (rewrite rev_length; reflexivity).
+replace (skipn (length l)) with (@skipn Cell (length (rev l))) by
+  (rewrite rev_length; reflexivity).
+rewrite firstn_app_3, skipn_app_3, rev_involutive.
+intros [eq0 eq1].
+elim eq0 using (K_dec_set Nat.eq_dec).
+elim eq1 using (K_dec_set State_dec).
+clear eq0 eq1.
 destruct ctx as [irf [rp rn] [wd we] iwf].
 reflexivity.
 Qed.
@@ -527,20 +505,33 @@ Local Open Scope thrist_scope.
 Notation "x ~~> y" := (MachineCode.T x y) (at level 70) : type_scope.
 Notation "x ->> y" := (Thrst MachineCode.T x y) (at level 70) : type_scope.
 
+(* A Bit Machine programs takes an inital state, x, and tries to produce a
+ * thrist of basic state transformations to some final state, y. However, a
+ * can potentially crash instead if it cannot execute successfully given the
+ * inital state.
+ *)
 Definition Program := forall x : State, option { y : State & x ->> y }.
 
-Definition crash : Program :=
-  fun x => None.
-
+(* The nop program has no basic instructions. *)
 Definition nop : Program :=
   fun x => Some (existT _ x []).
 
+(* For each basic instruction we define a program that executes only that
+ * single instruction.  For each instruction we have a correctness lemma
+ * that describes the result of the program when executed with an initial
+ * state that is legal for that instruction.
+ *)
+
+(* The newFrame instruction is legal to execute in any initial state.  We don't
+ * provide a correctness function for it since it can be evaluated inside Coq
+ * on any abstract input (i.e. it doesn't need any iota reductions).
+ *)
 Definition newFrame (n : nat) : Program :=
   fun x => Some (existT _ _ (MachineCode.NewFrame n x <| [])).
 
 Definition moveFrame : Program.
 intros s.
-destruct (MoveFrame_ctx s) as [P|];[left|right].
+destruct (MoveFrame_chk s) as [P|];[left|right].
 destruct P as [[l ctx] Hs].
 exact (existT _ _ (eq_nil Hs |> MachineCode.MoveFrame l ctx)).
 Defined.
@@ -554,13 +545,13 @@ Lemma moveFrame_correct : forall l ctx, moveFrame
 Proof.
 intros l ctx.
 unfold moveFrame.
-rewrite MoveFrame_ctx_correct.
+rewrite MoveFrame_chk_correct.
 reflexivity.
 Qed.
 
 Definition dropFrame : Program.
 intros s.
-destruct (DropFrame_ctx s) as [P|];[left|right].
+destruct (DropFrame_chk s) as [P|];[left|right].
 destruct P as [[rf ctx] Hs].
 exact (existT _ _ (eq_nil Hs |> MachineCode.DropFrame rf ctx)).
 Defined.
@@ -574,13 +565,13 @@ Lemma dropFrame_correct : forall rf ctx, dropFrame
 Proof.
 intros l ctx.
 unfold dropFrame.
-rewrite DropFrame_ctx_correct.
+rewrite DropFrame_chk_correct.
 reflexivity.
 Qed.
 
 Definition write (b : bool) : Program.
 intros s.
-destruct (Write_ctx s) as [P|];[left|right].
+destruct (Write_chk s) as [P|];[left|right].
 destruct P as [ctx Hs].
 exact (existT _ _ (eq_nil Hs |> MachineCode.Write b ctx)).
 Defined.
@@ -592,13 +583,13 @@ Lemma write_correct : forall b ctx, write b
 Proof.
 intros l ctx.
 unfold write.
-rewrite Write_ctx_correct.
+rewrite Write_chk_correct.
 reflexivity.
 Qed.
 
 Definition skip (n : nat) : Program.
 intros s.
-destruct (Skip_ctx n s) as [P|];[left|right].
+destruct (Skip_chk n s) as [P|];[left|right].
 destruct P as [ctx Hs].
 exact (existT _ _ (eq_nil Hs |> MachineCode.Skip n ctx)).
 Defined.
@@ -610,13 +601,13 @@ Lemma skip_correct : forall n ctx, skip n
 Proof.
 intros l ctx.
 unfold skip.
-rewrite Skip_ctx_correct.
+rewrite Skip_chk_correct.
 reflexivity.
 Qed.
 
 Definition copy (n : nat) : Program.
 intros s.
-destruct (Copy_ctx n s) as [P|];[left|right].
+destruct (Copy_chk n s) as [P|];[left|right].
 destruct P as [[l ctx] [_ Hs]].
 exact (existT _ _ (eq_nil Hs |> MachineCode.Copy l ctx)).
 Defined.
@@ -628,13 +619,13 @@ Lemma copy_correct : forall l ctx, copy (length l)
 Proof.
 intros l ctx.
 unfold copy.
-rewrite Copy_ctx_correct.
+rewrite Copy_chk_correct.
 reflexivity.
 Qed.
 
 Definition fwd (n : nat) : Program.
 intros s.
-destruct (Fwd_ctx n s) as [P|];[left|right].
+destruct (Fwd_chk n s) as [P|];[left|right].
 destruct P as [[l ctx] [_ Hs]].
 exact (existT _ _ (eq_nil Hs |> MachineCode.Fwd l ctx)).
 Defined.
@@ -646,13 +637,13 @@ Lemma fwd_correct : forall l ctx, fwd (length l)
 Proof.
 intros l ctx.
 unfold fwd.
-rewrite Fwd_ctx_correct.
+rewrite Fwd_chk_correct.
 reflexivity.
 Qed.
 
 Definition bwd (n : nat) : Program.
 intros s.
-destruct (Bwd_ctx n s) as [P|];[left|right].
+destruct (Bwd_chk n s) as [P|];[left|right].
 destruct P as [[l ctx] [_ Hs]].
 exact (existT _ _ (eq_nil Hs |> MachineCode.Bwd l ctx)).
 Defined.
@@ -664,10 +655,23 @@ Lemma bwd_correct : forall l ctx, bwd (length l)
 Proof.
 intros l ctx.
 unfold bwd.
-rewrite Bwd_ctx_correct.
+rewrite Bwd_chk_correct.
 reflexivity.
 Qed.
 
+(* The basic instruction crash always crashes the machine.  Crash doesn't
+ * appear in the MachineCode.T because there is no state that is can
+ * successfuly be executed in.  For the same reason it has no correctness
+ * lemma.
+ *)
+Definition crash : Program :=
+  fun x => None.
+
+(* There are two combinators for building larger programs from smaller ones:
+ * seq runs two programs, one after the other.  choice runs one of two programs
+ * depending on whether the Cell value under the cursor on the active read
+ * frame is a 0 or a 1.
+ *)
 Definition seq (p1 p2 : Program) : Program.
 intros x.
 destruct (p1 x) as [[y thr1]|];[|exact None].
@@ -685,11 +689,21 @@ Notation "p1 ||| p2" := (choice p1 p2) (at level 50, left associativity) : mc_sc
 
 Local Open Scope mc_scope.
 
+(* bump is notation for a program that is run where the active read frame's
+ * cursor is temporarily advanced.
+ *)
 Definition bump n p : Program := fwd n ;;; p ;;; bwd n.
 
+(* runMachine extracts the final state after executing a program, if
+ * successful.
+ *)
 Definition runMachine (p : Program) (s : State) : option State :=
 option_map (@projT1 _ _) (p s).
 
+
+(* The following lemma describe the behaviour of program cominators with
+ * runMachine.
+ *)
 Lemma runMachine_seq (p1 p2 : Program) (s : State) :
  runMachine (p1 ;;; p2) s = option_bind (runMachine p2) (runMachine p1 s).
 Proof.
