Coq/Util/List.v
@@ -1,4 +1,5 @@
 Require Export Coq.Lists.List.
+Require Import PeanoNat.
 
 Lemma repeat_S_tail {A} : forall (a : A) n, repeat a n ++ (a :: nil) = repeat a (S n).
 Proof.
@@ -18,3 +19,49 @@ rewrite IHn, repeat_S_tail.
 reflexivity.
 Qed.
 
+Lemma firstn_app_3 {A} (l1 l2 : list A) :
+  firstn (length l1) (l1 ++ l2) = l1.
+Proof.
+rewrite <- (Plus.plus_0_r (length l1)), firstn_app_2; cbn.
+apply app_nil_r.
+Qed.
+
+Lemma skipn_all {A} (l : list A) : skipn (length l) l = nil.
+Proof.
+apply (app_inv_head (firstn (length l) l)).
+rewrite firstn_skipn, firstn_all, app_nil_r; auto.
+Qed.
+
+Lemma skipn_all2 {A} n (l : list A) : length l <= n -> skipn n l = nil.
+Proof.
+intros Hn.
+apply (app_inv_head (firstn n l)).
+rewrite firstn_skipn, firstn_all2, app_nil_r; auto.
+Qed.
+
+Lemma skipn_app {A} (n : nat) : forall (l1 l2 : list A),
+       skipn n (l1 ++ l2) = skipn n l1 ++ skipn (n - length l1) l2.
+Proof.
+induction n.
+ reflexivity.
+destruct l1.
+ reflexivity.
+apply IHn.
+Qed.
+
+Lemma skipn_app_2 {A} (n : nat) : forall (l1 l2 : list A),
+       skipn (length l1 + n) (l1 ++ l2) = skipn n l2.
+Proof.
+intros l1 l2.
+rewrite skipn_app, Minus.minus_plus, skipn_all2; auto with arith.
+Qed.
+
+Lemma skipn_app_3 {A} (l1 l2 : list A) :
+  skipn (length l1) (l1 ++ l2) = l2.
+Proof.
+apply (app_inv_head l1).
+rewrite <- (firstn_app_3 l1 l2) at 1.
+apply firstn_skipn.
+Qed.
+
+Definition nat_sum : list nat -> nat := fold_right plus O.
